Temporarily remove algIDs.

src/X509.Base.fst
@@ -10,22 +10,27 @@ open FStar.Integers
 
 module B32 = FStar.Bytes
 
-type supported_crypto_alg_t =
-| AlgID_ECDSA_P256
-| AlgID_Ed25519
+(* Disabling them for now *)
+// type supported_crypto_alg_t =
+// | AlgID_ECDSA_P256
+// | AlgID_Ed25519
 
 unfold
 let pubkey_len
-  (pubkey_alg: supported_crypto_alg_t)
-= match pubkey_alg with
-  | AlgID_ECDSA_P256 -> 32ul
-  | AlgID_Ed25519    -> 32ul
+  // (pubkey_alg: supported_crypto_alg_t)
+=
+  // match pubkey_alg with
+  // | AlgID_ECDSA_P256 -> 32ul
+  // | AlgID_Ed25519    ->
+  32ul
 
 unfold
 let pubkey_t
-  (pubkey_alg: supported_crypto_alg_t)
-= match pubkey_alg with
-  | AlgID_ECDSA_P256 -> datatype_of_asn1_type BIT_STRING
-  | AlgID_Ed25519    -> bs: datatype_of_asn1_type BIT_STRING
+  // (pubkey_alg: supported_crypto_alg_t)
+=
+  // match pubkey_alg with
+  // | AlgID_ECDSA_P256 -> datatype_of_asn1_type BIT_STRING
+  // | AlgID_Ed25519    ->
+  bs: datatype_of_asn1_type BIT_STRING
                      { bs.bs_len == 33ul /\
                        bs.bs_unused_bits == 0ul}
