src/X509.BasicFields.SubjectPublicKeyInfo.fst
@@ -18,135 +18,143 @@ open FStar.Integers
 
 //inline_for_extraction
 type subjectPublicKeyInfo_t
-  (alg: supported_crypto_alg_t)
-= { subjectPubKey_alg : algorithmIdentifier_t_inbound alg;
-    subjectPubKey     : pubkey_t alg }
+  // (alg: supported_crypto_alg_t)
+= { subjectPubKey_alg : algorithmIdentifier_t_inbound;
+    subjectPubKey     : pubkey_t }
 
 let filter_subjectPublicKeyInfo_t'
-  (alg: supported_crypto_alg_t)
-  (x: (algorithmIdentifier_t_inbound alg) `tuple2` (datatype_of_asn1_type BIT_STRING))
+  // (alg: supported_crypto_alg_t)
+  (x: (algorithmIdentifier_t_inbound) `tuple2` (datatype_of_asn1_type BIT_STRING))
 : GTot bool
-= match alg with
-  | AlgID_ECDSA_P256 -> true
-  | AlgID_Ed25519    -> (snd x).bs_len = 33ul &&
-                  (snd x).bs_unused_bits = 0ul
+=
+  // match alg with
+  // | AlgID_ECDSA_P256 -> true
+  // | AlgID_Ed25519    ->
+  (snd x).bs_len = 33ul &&
+  (snd x).bs_unused_bits = 0ul
 
 /// tuple repr
 
 unfold
 let subjectPublicKeyInfo_t'
-  (alg: supported_crypto_alg_t)
-= parse_filter_refine (filter_subjectPublicKeyInfo_t' alg)
+  // (alg: supported_crypto_alg_t)
+= parse_filter_refine (filter_subjectPublicKeyInfo_t')
 
 let synth_subjectPublicKeyInfo_t
-  (alg: supported_crypto_alg_t)
-  (x': subjectPublicKeyInfo_t' alg)
-: GTot (subjectPublicKeyInfo_t alg)
+  // (alg: supported_crypto_alg_t)
+  (x': subjectPublicKeyInfo_t')
+: GTot (subjectPublicKeyInfo_t)
 = { subjectPubKey_alg = fst x';
     subjectPubKey     = snd x' }
 
 
 let synth_subjectPublicKeyInfo_t'
-  (alg: supported_crypto_alg_t)
-  (x: subjectPublicKeyInfo_t alg)
-: Tot (x': subjectPublicKeyInfo_t' alg { x == synth_subjectPublicKeyInfo_t alg x' })
+  // (alg: supported_crypto_alg_t)
+  (x: subjectPublicKeyInfo_t)
+: Tot (x': subjectPublicKeyInfo_t' { x == synth_subjectPublicKeyInfo_t x' })
 = (x.subjectPubKey_alg , x.subjectPubKey)
 
 let parse_subjectPublicKeyInfo
-  (alg: supported_crypto_alg_t)
-: parser _ (subjectPublicKeyInfo_t alg)
-= parse_algorithmIdentifier_sequence_TLV alg
+  // (alg: supported_crypto_alg_t)
+: parser _ (subjectPublicKeyInfo_t)
+= parse_algorithmIdentifier_sequence_TLV
   `nondep_then`
   parse_asn1_TLV_of_type BIT_STRING
   `parse_filter`
-  filter_subjectPublicKeyInfo_t' alg
+  filter_subjectPublicKeyInfo_t'
   `parse_synth`
-  synth_subjectPublicKeyInfo_t alg
+  synth_subjectPublicKeyInfo_t
 
 let serialize_subjectPublicKeyInfo
-  (alg: supported_crypto_alg_t)
-: serializer (parse_subjectPublicKeyInfo alg)
+  // (alg: supported_crypto_alg_t)
+: serializer (parse_subjectPublicKeyInfo)
 = serialize_synth
-  (* p1 *) (parse_algorithmIdentifier_sequence_TLV alg
+  (* p1 *) (parse_algorithmIdentifier_sequence_TLV
             `nondep_then`
             parse_asn1_TLV_of_type BIT_STRING
             `parse_filter`
-            filter_subjectPublicKeyInfo_t' alg)
-  (* f2 *) (synth_subjectPublicKeyInfo_t alg)
-  (* s1 *) (serialize_algorithmIdentifier_sequence_TLV alg
+            filter_subjectPublicKeyInfo_t')
+  (* f2 *) (synth_subjectPublicKeyInfo_t)
+  (* s1 *) (serialize_algorithmIdentifier_sequence_TLV
             `serialize_nondep_then`
             serialize_asn1_TLV_of_type BIT_STRING
             `serialize_filter`
-            filter_subjectPublicKeyInfo_t' alg)
-  (* g1 *) (synth_subjectPublicKeyInfo_t' alg)
+            filter_subjectPublicKeyInfo_t')
+  (* g1 *) (synth_subjectPublicKeyInfo_t')
   (* prf*) ()
 
 let lemma_serialize_subjectPublicKeyInfo_unfold
-  (alg: supported_crypto_alg_t)
-  (x: subjectPublicKeyInfo_t alg)
+  // (alg: supported_crypto_alg_t)
+  (x: subjectPublicKeyInfo_t)
 : Lemma (
-  serialize (serialize_subjectPublicKeyInfo alg) x ==
-  serialize (serialize_algorithmIdentifier_sequence_TLV alg) x.subjectPubKey_alg
+  serialize (serialize_subjectPublicKeyInfo) x ==
+  serialize (serialize_algorithmIdentifier_sequence_TLV) x.subjectPubKey_alg
   `Seq.append`
   serialize (serialize_asn1_TLV_of_type BIT_STRING) x.subjectPubKey
 )
 = serialize_nondep_then_eq
-  (* s1 *) (serialize_algorithmIdentifier_sequence_TLV alg)
+  (* s1 *) (serialize_algorithmIdentifier_sequence_TLV)
   (* s2 *) (serialize_asn1_TLV_of_type BIT_STRING)
-  (* in *) (synth_subjectPublicKeyInfo_t' alg x);
+  (* in *) (synth_subjectPublicKeyInfo_t' x);
   serialize_synth_eq
-  (* p1 *) (parse_algorithmIdentifier_sequence_TLV alg
+  (* p1 *) (parse_algorithmIdentifier_sequence_TLV
             `nondep_then`
             parse_asn1_TLV_of_type BIT_STRING
             `parse_filter`
-            filter_subjectPublicKeyInfo_t' alg)
-  (* f2 *) (synth_subjectPublicKeyInfo_t alg)
-  (* s1 *) (serialize_algorithmIdentifier_sequence_TLV alg
+            filter_subjectPublicKeyInfo_t')
+  (* f2 *) (synth_subjectPublicKeyInfo_t)
+  (* s1 *) (serialize_algorithmIdentifier_sequence_TLV
             `serialize_nondep_then`
             serialize_asn1_TLV_of_type BIT_STRING
             `serialize_filter`
-            filter_subjectPublicKeyInfo_t' alg)
-  (* g1 *) (synth_subjectPublicKeyInfo_t' alg)
+            filter_subjectPublicKeyInfo_t')
+  (* g1 *) (synth_subjectPublicKeyInfo_t')
   (* prf*) ()
   (* in *) x
 
 let lemma_serialize_subjectPublicKeyInfo_size
-  (alg: supported_crypto_alg_t)
-  (x: subjectPublicKeyInfo_t alg)
+  // (alg: supported_crypto_alg_t)
+  (x: subjectPublicKeyInfo_t)
 : Lemma (
-  Seq.length (serialize (serialize_subjectPublicKeyInfo alg) x) ==
-  Seq.length (serialize (serialize_algorithmIdentifier_sequence_TLV alg) x.subjectPubKey_alg) +
+  Seq.length (serialize (serialize_subjectPublicKeyInfo) x) ==
+  Seq.length (serialize (serialize_algorithmIdentifier_sequence_TLV) x.subjectPubKey_alg) +
   Seq.length (serialize (serialize_asn1_TLV_of_type BIT_STRING) x.subjectPubKey)
 )
-= lemma_serialize_subjectPublicKeyInfo_unfold alg x
+= lemma_serialize_subjectPublicKeyInfo_unfold x
 
 let subjectPublicKeyInfo_t_inbound
-  (alg: supported_crypto_alg_t)
-= inbound_sequence_value_of (serialize_subjectPublicKeyInfo alg)
+  // (alg: supported_crypto_alg_t)
+= inbound_sequence_value_of (serialize_subjectPublicKeyInfo)
 
 /// TLV
 ///
 let parse_subjectPublicKeyInfo_sequence_TLV
-  (alg: supported_crypto_alg_t)
-: parser _ (subjectPublicKeyInfo_t_inbound alg)
-= parse_asn1_sequence_TLV (serialize_subjectPublicKeyInfo alg)
+  // (alg: supported_crypto_alg_t)
+// : parser _ (subjectPublicKeyInfo_t_inbound)
+=
+  subjectPublicKeyInfo_t_inbound
+  `coerce_parser`
+  parse_asn1_sequence_TLV (serialize_subjectPublicKeyInfo)
 
 let serialize_subjectPublicKeyInfo_sequence_TLV
-  (alg: supported_crypto_alg_t)
-: serializer (parse_subjectPublicKeyInfo_sequence_TLV alg)
-= serialize_asn1_sequence_TLV (serialize_subjectPublicKeyInfo alg)
+  // (alg: supported_crypto_alg_t)
+// : serializer (parse_subjectPublicKeyInfo_sequence_TLV)
+= coerce_parser_serializer
+    parse_subjectPublicKeyInfo_sequence_TLV
+    (serialize_asn1_sequence_TLV (serialize_subjectPublicKeyInfo))
+    ()
 
 let lemma_serialize_subjectPublicKeyInfo_sequence_TLV_unfold
-  (alg: supported_crypto_alg_t)
-  (x: subjectPublicKeyInfo_t_inbound alg)
-: Lemma ( predicate_serialize_asn1_sequence_TLV_unfold (serialize_subjectPublicKeyInfo alg) x )
-= lemma_serialize_asn1_sequence_TLV_unfold (serialize_subjectPublicKeyInfo alg) x
+  // (alg: supported_crypto_alg_t)
+  (x: subjectPublicKeyInfo_t_inbound)
+: Lemma ( predicate_serialize_asn1_sequence_TLV_unfold (serialize_subjectPublicKeyInfo) x )
+= lemma_serialize_asn1_sequence_TLV_unfold (serialize_subjectPublicKeyInfo) x
 
 let lemma_serialize_subjectPublicKeyInfo_sequence_TLV_size
-  (alg: supported_crypto_alg_t)
-  (x: subjectPublicKeyInfo_t_inbound alg)
-: Lemma ( predicate_serialize_asn1_sequence_TLV_size (serialize_subjectPublicKeyInfo alg) x )
-= lemma_serialize_asn1_sequence_TLV_size (serialize_subjectPublicKeyInfo alg) x
+  // (alg: supported_crypto_alg_t)
+  (x: subjectPublicKeyInfo_t_inbound)
+: Lemma ( predicate_serialize_asn1_sequence_TLV_size (serialize_subjectPublicKeyInfo) x )
+= lemma_serialize_asn1_sequence_TLV_size (serialize_subjectPublicKeyInfo) x
 
 (* NOTE: For a subjectPublicKeyInfo for Ed25519, it consists
          1) a 1-byte tag
@@ -172,21 +180,23 @@ let lemma_serialize_subjectPublicKeyInfo_sequence_TLV_size
 
 #push-options "--z3rlimit 32"
 let lemma_serialize_subjectPublicKeyInfo_sequence_TLV_size_exact
-  (alg: supported_crypto_alg_t {alg == AlgID_Ed25519})
-  (x: subjectPublicKeyInfo_t_inbound alg)
+  // (alg: supported_crypto_alg_t {alg == AlgID_Ed25519})
+  (x: subjectPublicKeyInfo_t_inbound)
 : Lemma (
-  match alg with
-  | AlgID_Ed25519   -> ( length_of_opaque_serialization (serialize_subjectPublicKeyInfo_sequence_TLV alg) x == 44 )
+  // match alg with
+  // | AlgID_Ed25519   ->
+  ( length_of_opaque_serialization (serialize_subjectPublicKeyInfo_sequence_TLV) x == 44 )
 )
 =
-  match alg with
-  | AlgID_Ed25519   -> ( (* reveal the SEQUENCE envelop *)
-                   lemma_serialize_subjectPublicKeyInfo_sequence_TLV_unfold alg x;
-                   lemma_serialize_subjectPublicKeyInfo_sequence_TLV_size   alg x;
+  // match alg with
+  // | AlgID_Ed25519   ->
+                     ( (* reveal the SEQUENCE envelop *)
+                   lemma_serialize_subjectPublicKeyInfo_sequence_TLV_unfold x;
+                   lemma_serialize_subjectPublicKeyInfo_sequence_TLV_size   x;
                      (* reveal the SEQUENCE body *)
-                     lemma_serialize_subjectPublicKeyInfo_size alg x;
-                     (**) lemma_serialize_algorithmIdentifier_sequence_TLV_size_exact alg x.subjectPubKey_alg;
-                     assert ( let bs: pubkey_t AlgID_Ed25519 = x.subjectPubKey in
+                     lemma_serialize_subjectPublicKeyInfo_size x;
+                     (**) lemma_serialize_algorithmIdentifier_sequence_TLV_size_exact x.subjectPubKey_alg;
+                     assert ( let bs: pubkey_t = x.subjectPubKey in
                               length_of_asn1_primitive_TLV bs == 35 );
                      () )
 #pop-options
@@ -196,57 +206,60 @@ let lemma_serialize_subjectPublicKeyInfo_sequence_TLV_size_exact
 
 inline_for_extraction
 let serialize32_subjectPublicKeyInfo_backwards
-  (alg: supported_crypto_alg_t)
-: serializer32_backwards (serialize_subjectPublicKeyInfo alg)
+  // (alg: supported_crypto_alg_t)
+: serializer32_backwards (serialize_subjectPublicKeyInfo)
 = serialize32_synth_backwards
-  (* ls *) (serialize32_algorithmIdentifier_sequence_TLV_backwards alg
+  (* ls *) (serialize32_algorithmIdentifier_sequence_TLV_backwards
             `serialize32_nondep_then_backwards`
             serialize32_asn1_TLV_backwards_of_type BIT_STRING
             `serialize32_filter_backwards`
-            filter_subjectPublicKeyInfo_t' alg)
-  (* f2 *) (synth_subjectPublicKeyInfo_t alg)
-  (* g1 *) (synth_subjectPublicKeyInfo_t' alg)
-  (* g1'*) (synth_subjectPublicKeyInfo_t' alg)
+            filter_subjectPublicKeyInfo_t')
+  (* f2 *) (synth_subjectPublicKeyInfo_t)
+  (* g1 *) (synth_subjectPublicKeyInfo_t')
+  (* g1'*) (synth_subjectPublicKeyInfo_t')
   (* prf*) ()
 
 inline_for_extraction
 let serialize32_subjectPublicKeyInfo_sequence_TLV_backwards
-  (alg: supported_crypto_alg_t)
-: serializer32_backwards (serialize_subjectPublicKeyInfo_sequence_TLV alg)
-= serialize32_asn1_sequence_TLV_backwards
-  (* ls *) (serialize32_subjectPublicKeyInfo_backwards alg)
-
+  // (alg: supported_crypto_alg_t)
+: serializer32_backwards (serialize_subjectPublicKeyInfo_sequence_TLV)
+= coerce_serializer32_backwards
+    (serialize_subjectPublicKeyInfo_sequence_TLV)
+    (serialize32_asn1_sequence_TLV_backwards
+     (* ls *) (serialize32_subjectPublicKeyInfo_backwards))
+    ()
 (* helpers *)
-let _ = assert (length_of_oid OID_EC_GRP_SECP256R1 == 6)
 
 module B32 = FStar.Bytes
 open X509.Crypto.AlgorithmIdentifier
 let subjectPublicKeyInfo_raw_t
-  (alg: supported_crypto_alg_t{alg == AlgID_Ed25519})
-= match alg with
-  | AlgID_Ed25519   -> B32.lbytes32 32ul
+  // (alg: supported_crypto_alg_t{alg == AlgID_Ed25519})
+=
+  // match alg with
+  // | AlgID_Ed25519   ->
+  B32.lbytes32 32ul
 
 #push-options "--z3rlimit 16 --fuel 0 --ifuel 0"
 let x509_get_subjectPublicKeyInfo
-  (pubkey_alg: supported_crypto_alg_t {pubkey_alg == AlgID_Ed25519} )
+  // (pubkey_alg: supported_crypto_alg_t {pubkey_alg == AlgID_Ed25519} )
   (pubkey: B32.lbytes32 32ul)
-: Tot (subjectPublicKeyInfo_t_inbound pubkey_alg)
+: Tot (subjectPublicKeyInfo_t_inbound)
 =
   lemma_trivial_bit_string_is_valid 33ul pubkey;
-  let pubkey_bs: pubkey_t pubkey_alg = Mkbit_string_t 33ul 0ul pubkey in
+  let pubkey_bs: pubkey_t  = Mkbit_string_t 33ul 0ul pubkey in
 
-  if (pubkey_alg = AlgID_Ed25519) then
-  ( let alg_id: algorithmIdentifier_t_inbound pubkey_alg = x509_get_algorithmIdentifier pubkey_alg in
-    (* Prf *) lemma_serialize_algorithmIdentifier_sequence_TLV_size_exact pubkey_alg alg_id;
+  // if (pubkey_alg = AlgID_Ed25519) then
+  ( let alg_id: algorithmIdentifier_t_inbound = x509_get_algorithmIdentifier () in
+    (* Prf *) lemma_serialize_algorithmIdentifier_sequence_TLV_size_exact alg_id;
 
-    let aliasPublicKeyInfo: subjectPublicKeyInfo_t pubkey_alg = {
+    let aliasPublicKeyInfo: subjectPublicKeyInfo_t = {
        subjectPubKey_alg = alg_id;
        subjectPubKey     = pubkey_bs
     } in
-    (* Prf *) lemma_serialize_subjectPublicKeyInfo_size pubkey_alg aliasPublicKeyInfo;
+    (* Prf *) lemma_serialize_subjectPublicKeyInfo_size aliasPublicKeyInfo;
     (* Prf *) (**) lemma_serialize_asn1_bit_string_TLV_size aliasPublicKeyInfo.subjectPubKey;
 
     (* return *) aliasPublicKeyInfo )
-  else
-  ( false_elim() )
+  // else
+  // ( false_elim() )
 #pop-options
