src/X509.Crypto.AlgorithmIdentifier.fst
@@ -28,162 +28,180 @@ type algorithmIdentifier_Ed25519_t = {
 }
 
 let algorithmIdentifier_t
-  (alg: supported_crypto_alg_t)
-= match alg with
-  | AlgID_ECDSA_P256 -> algorithmIdentifier_ECDSA_P256_t
-  | AlgID_Ed25519    -> algorithmIdentifier_Ed25519_t
+  // (alg: supported_crypto_alg_t)
+= algorithmIdentifier_Ed25519_t
+  // match alg with
+  // | AlgID_ECDSA_P256 -> algorithmIdentifier_ECDSA_P256_t
+  // | AlgID_Ed25519    -> algorithmIdentifier_Ed25519_t
 
 private
 let algorithmIdentifier_t'_aux
-  (alg: supported_crypto_alg_t)
-= match alg with
-  | AlgID_ECDSA_P256 -> tuple2 (datatype_of_asn1_type OID) (datatype_of_asn1_type OID)
-  | AlgID_Ed25519    -> datatype_of_asn1_type OID
+  // (alg: supported_crypto_alg_t)
+=
+  // match alg with
+  // | AlgID_ECDSA_P256 -> tuple2 (datatype_of_asn1_type OID) (datatype_of_asn1_type OID)
+  // | AlgID_Ed25519    ->
+  datatype_of_asn1_type OID
 
 /// tuple repr
 let filter_algorithmIdentifier_t'
-  (alg: supported_crypto_alg_t)
-  (x': algorithmIdentifier_t'_aux alg)
+  // (alg: supported_crypto_alg_t)
+  (x': algorithmIdentifier_t'_aux)
 : GTot bool
-= match alg with
-  | AlgID_ECDSA_P256 -> ( let x' = x' <: tuple2 (datatype_of_asn1_type OID) (datatype_of_asn1_type OID) in
-                    fst x' = OID_EC_ALG_UNRESTRICTED &&
-                    snd x' = OID_EC_GRP_SECP256R1 )
-  | AlgID_Ed25519    -> ( let x' = x'<: datatype_of_asn1_type OID in
+=
+  // match alg with
+  // | AlgID_ECDSA_P256 -> ( let x' = x' <: tuple2 (datatype_of_asn1_type OID) (datatype_of_asn1_type OID) in
+  //                   fst x' = OID_EC_ALG_UNRESTRICTED &&
+  //                   snd x' = OID_EC_GRP_SECP256R1 )
+  // | AlgID_Ed25519    ->
+  ( let x' = x'<: datatype_of_asn1_type OID in
                     x' = OID_ED25519 )
 
 let algorithmIdentifier_t'
-  (alg: supported_crypto_alg_t)
-= parse_filter_refine (filter_algorithmIdentifier_t' alg)
+  // (alg: supported_crypto_alg_t)
+= parse_filter_refine (filter_algorithmIdentifier_t')
 
 /// tuple repr -> record repr
 let synth_algorithmIdentifier_t
-  (alg: supported_crypto_alg_t)
-  (x': algorithmIdentifier_t' alg)
-: GTot (algorithmIdentifier_t alg)
-= match alg with
-  | AlgID_ECDSA_P256 -> ( let x' = x' <: tuple2 (datatype_of_asn1_type OID) (datatype_of_asn1_type OID) in
-                    { alg_id_oid_ecdsa = fst x';
-                      alg_id_oid_p256  = snd x' } )
-  | AlgID_Ed25519    -> ( let x' = x' <: datatype_of_asn1_type OID in
+  // (alg: supported_crypto_alg_t)
+  (x': algorithmIdentifier_t')
+: GTot (algorithmIdentifier_t)
+=
+  // match alg with
+  // | AlgID_ECDSA_P256 -> ( let x' = x' <: tuple2 (datatype_of_asn1_type OID) (datatype_of_asn1_type OID) in
+  //                   { alg_id_oid_ecdsa = fst x';
+  //                     alg_id_oid_p256  = snd x' } )
+  // | AlgID_Ed25519    ->
+  ( let x' = x' <: datatype_of_asn1_type OID in
                     { algID_ed25519 = x' } )
 
 /// record repr -> tuple repr
 
 inline_for_extraction noextract
 let synth_algorithmIdentifier_t'
-  (alg: supported_crypto_alg_t)
-  (x: algorithmIdentifier_t alg)
-: Tot (x': algorithmIdentifier_t' alg { x == synth_algorithmIdentifier_t alg x' })
-= match alg with
-  | AlgID_ECDSA_P256 -> ( let x = x <: algorithmIdentifier_ECDSA_P256_t in
-                    ((x.alg_id_oid_ecdsa <: datatype_of_asn1_type OID),
-                     (x.alg_id_oid_p256  <: datatype_of_asn1_type OID)) )
-  | AlgID_Ed25519    -> ( let x = x<: algorithmIdentifier_Ed25519_t in
+  // (alg: supported_crypto_alg_t)
+  (x: algorithmIdentifier_t)
+: Tot (x': algorithmIdentifier_t' { x == synth_algorithmIdentifier_t x' })
+=
+  // match alg with
+  // | AlgID_ECDSA_P256 -> ( let x = x <: algorithmIdentifier_ECDSA_P256_t in
+  //                   ((x.alg_id_oid_ecdsa <: datatype_of_asn1_type OID),
+  //                    (x.alg_id_oid_p256  <: datatype_of_asn1_type OID)) )
+  // | AlgID_Ed25519    ->
+  ( let x = x<: algorithmIdentifier_Ed25519_t in
                     x.algID_ed25519 )
 
 let parse_algorithmIdentifier_kind
-  (alg: supported_crypto_alg_t)
+  // (alg: supported_crypto_alg_t)
 : parser_kind
-= match alg with
-  | AlgID_ECDSA_P256 -> ( parse_asn1_TLV_kind_of_type OID
-                    `and_then_kind`
-                    parse_asn1_TLV_kind_of_type OID )
-  | AlgID_Ed25519    -> ( parse_asn1_TLV_kind_of_type OID )
+=
+  // match alg with
+  // | AlgID_ECDSA_P256 -> ( parse_asn1_TLV_kind_of_type OID
+  //                   `and_then_kind`
+  //                   parse_asn1_TLV_kind_of_type OID )
+  // | AlgID_Ed25519    ->
+  ( parse_asn1_TLV_kind_of_type OID )
 
 /// sequence value (body) parser
 let parse_algorithmIdentifier
-  (alg: supported_crypto_alg_t)
-: parser (parse_algorithmIdentifier_kind alg) (algorithmIdentifier_t alg)
-= match alg with
-  | AlgID_ECDSA_P256 -> ( parse_asn1_TLV_of_type OID
-                    `nondep_then`
-                    parse_asn1_TLV_of_type OID
+  // (alg: supported_crypto_alg_t)
+: parser (parse_algorithmIdentifier_kind) (algorithmIdentifier_t)
+=
+  // match alg with
+  // | AlgID_ECDSA_P256 -> ( parse_asn1_TLV_of_type OID
+  //                   `nondep_then`
+  //                   parse_asn1_TLV_of_type OID
+  //                   `parse_filter`
+  //                   filter_algorithmIdentifier_t' alg
+  //                   `parse_synth`
+  //                   synth_algorithmIdentifier_t alg )
+  // | AlgID_Ed25519    ->
+  ( parse_asn1_TLV_of_type OID
                     `parse_filter`
-                    filter_algorithmIdentifier_t' alg
+                    filter_algorithmIdentifier_t'
                     `parse_synth`
-                    synth_algorithmIdentifier_t alg )
-  | AlgID_Ed25519    -> ( parse_asn1_TLV_of_type OID
-                    `parse_filter`
-                    filter_algorithmIdentifier_t' alg
-                    `parse_synth`
-                    synth_algorithmIdentifier_t alg)
+                    synth_algorithmIdentifier_t)
 
 /// sequence value serializer
 let serialize_algorithmIdentifier
-  (alg: supported_crypto_alg_t)
-: serializer (parse_algorithmIdentifier alg)
-= match alg with
-  | AlgID_ECDSA_P256 -> ( serialize_synth
-                    (* p1 *) (parse_asn1_TLV_of_type OID
-                              `nondep_then`
-                              parse_asn1_TLV_of_type OID
-                              `parse_filter`
-                              filter_algorithmIdentifier_t' alg)
-                    (* f2 *) (synth_algorithmIdentifier_t alg)
-                    (* s1 *) (serialize_asn1_TLV_of_type OID
-                              `serialize_nondep_then`
-                              serialize_asn1_TLV_of_type OID
-                              `serialize_filter`
-                              filter_algorithmIdentifier_t' alg)
-                    (* g1 *) (synth_algorithmIdentifier_t' alg)
-                    (* prf*) () )
+  // (alg: supported_crypto_alg_t)
+: serializer (parse_algorithmIdentifier)
+=
+  // match alg with
+  // | AlgID_ECDSA_P256 -> ( serialize_synth
+  //                   (* p1 *) (parse_asn1_TLV_of_type OID
+  //                             `nondep_then`
+  //                             parse_asn1_TLV_of_type OID
+  //                             `parse_filter`
+  //                             filter_algorithmIdentifier_t' alg)
+  //                   (* f2 *) (synth_algorithmIdentifier_t alg)
+  //                   (* s1 *) (serialize_asn1_TLV_of_type OID
+  //                             `serialize_nondep_then`
+  //                             serialize_asn1_TLV_of_type OID
+  //                             `serialize_filter`
+  //                             filter_algorithmIdentifier_t' alg)
+  //                   (* g1 *) (synth_algorithmIdentifier_t' alg)
+  //                   (* prf*) () )
 
-  | AlgID_Ed25519    -> ( serialize_synth
+  // | AlgID_Ed25519    ->
+                           ( serialize_synth
                     (* p1 *) (parse_asn1_TLV_of_type OID
                               `parse_filter`
-                              filter_algorithmIdentifier_t' alg)
-                    (* f2 *) (synth_algorithmIdentifier_t alg)
+                              filter_algorithmIdentifier_t')
+                    (* f2 *) (synth_algorithmIdentifier_t)
                     (* s1 *) (serialize_asn1_TLV_of_type OID
                               `serialize_filter`
-                              filter_algorithmIdentifier_t' alg)
-                    (* g1 *) (synth_algorithmIdentifier_t' alg)
+                              filter_algorithmIdentifier_t')
+                    (* g1 *) (synth_algorithmIdentifier_t')
                     (* prf*) () )
 
 /// lemma: unfold sequence value serializer
 let lemma_serialize_algorithmIdentifier_unfold
-  (alg: supported_crypto_alg_t)
-  (x: algorithmIdentifier_t alg)
+  // (alg: supported_crypto_alg_t)
+  (x: algorithmIdentifier_t)
 : Lemma (
-  match alg with
-  | AlgID_ECDSA_P256 -> ( serialize (serialize_algorithmIdentifier alg) x ==
-                    serialize (serialize_asn1_TLV_of_type OID) OID_EC_ALG_UNRESTRICTED
-                    `Seq.append`
-                    serialize (serialize_asn1_TLV_of_type OID) OID_EC_GRP_SECP256R1 )
-  | AlgID_Ed25519    -> ( serialize (serialize_algorithmIdentifier alg) x ==
+  // match alg with
+  // | AlgID_ECDSA_P256 -> ( serialize (serialize_algorithmIdentifier alg) x ==
+  //                   serialize (serialize_asn1_TLV_of_type OID) OID_EC_ALG_UNRESTRICTED
+  //                   `Seq.append`
+  //                   serialize (serialize_asn1_TLV_of_type OID) OID_EC_GRP_SECP256R1 )
+  // | AlgID_Ed25519    ->
+                   ( serialize (serialize_algorithmIdentifier) x ==
                     serialize (serialize_asn1_TLV_of_type OID) OID_ED25519 /\
-                    length_of_opaque_serialization (serialize_algorithmIdentifier alg) x ==
+                    length_of_opaque_serialization (serialize_algorithmIdentifier) x ==
                     5
                     ))
-= match alg with
-  | AlgID_ECDSA_P256 -> ( serialize_nondep_then_eq
-                    (* s1 *) (serialize_asn1_TLV_of_type OID)
-                    (* s2 *) (serialize_asn1_TLV_of_type OID)
-                    (* in *) (synth_algorithmIdentifier_t' alg x);
-                    serialize_synth_eq
+=
+  // match alg with
+  // | AlgID_ECDSA_P256 -> ( serialize_nondep_then_eq
+  //                   (* s1 *) (serialize_asn1_TLV_of_type OID)
+  //                   (* s2 *) (serialize_asn1_TLV_of_type OID)
+  //                   (* in *) (synth_algorithmIdentifier_t' alg x);
+  //                   serialize_synth_eq
+  //                   (* p1 *) (parse_asn1_TLV_of_type OID
+  //                             `nondep_then`
+  //                             parse_asn1_TLV_of_type OID
+  //                             `parse_filter`
+  //                             filter_algorithmIdentifier_t' alg)
+  //                   (* f2 *) (synth_algorithmIdentifier_t alg)
+  //                   (* s1 *) (serialize_asn1_TLV_of_type OID
+  //                             `serialize_nondep_then`
+  //                             serialize_asn1_TLV_of_type OID
+  //                             `serialize_filter`
+  //                             filter_algorithmIdentifier_t' alg)
+  //                   (* g1 *) (synth_algorithmIdentifier_t' alg)
+  //                   (* prf*) ()
+  //                   (* in *) x )
+  // | AlgID_Ed25519    ->
+                          ( serialize_synth_eq
                     (* p1 *) (parse_asn1_TLV_of_type OID
-                              `nondep_then`
-                              parse_asn1_TLV_of_type OID
                               `parse_filter`
-                              filter_algorithmIdentifier_t' alg)
-                    (* f2 *) (synth_algorithmIdentifier_t alg)
-                    (* s1 *) (serialize_asn1_TLV_of_type OID
-                              `serialize_nondep_then`
-                              serialize_asn1_TLV_of_type OID
-                              `serialize_filter`
-                              filter_algorithmIdentifier_t' alg)
-                    (* g1 *) (synth_algorithmIdentifier_t' alg)
-                    (* prf*) ()
-                    (* in *) x )
-  | AlgID_Ed25519    -> ( serialize_synth_eq
-                    (* p1 *) (parse_asn1_TLV_of_type OID
-                              `parse_filter`
-                              filter_algorithmIdentifier_t' alg)
-                    (* f2 *) (synth_algorithmIdentifier_t alg)
+                              filter_algorithmIdentifier_t')
+                    (* f2 *) (synth_algorithmIdentifier_t)
                     (* s1 *) (serialize_asn1_TLV_of_type OID
                               `serialize_filter`
-                              filter_algorithmIdentifier_t' alg)
-                    (* g1 *) (synth_algorithmIdentifier_t' alg)
+                              filter_algorithmIdentifier_t')
+                    (* g1 *) (synth_algorithmIdentifier_t')
                     (* prf*) ()
                     (* in *) x;
                     assert_norm (length_of_asn1_primitive_TLV OID_ED25519 == 5) )
@@ -192,83 +210,96 @@ let lemma_serialize_algorithmIdentifier_unfold
 
 
 let lemma_serialize_algorithmIdentifier_size
-  (alg: supported_crypto_alg_t)
-  (x: algorithmIdentifier_t alg)
+  // (alg: supported_crypto_alg_t)
+  (x: algorithmIdentifier_t)
 : Lemma (
-  match alg with (* FIXME *)
+  // match alg with
   // | AlgID_ECDSA_P256 -> ( let x = x <: algorithmIdentifier_ECDSA_P256_t in
   //                   Seq.length (serialize (serialize_algorithmIdentifier alg) x) ==
   //                   length_of_asn1_primitive_TLV x.alg_id_oid_ecdsa +
   //                   length_of_asn1_primitive_TLV x.alg_id_oid_p256 )
-  | AlgID_Ed25519    -> ( let x = x <: algorithmIdentifier_Ed25519_t in
-                    Seq.length (serialize (serialize_algorithmIdentifier alg) x) ==
+  // | AlgID_Ed25519    ->
+                   ( let x = x <: algorithmIdentifier_Ed25519_t in
+                    Seq.length (serialize (serialize_algorithmIdentifier) x) ==
                     5 )
                     //length_of_asn1_primitive_TLV x.algID_ed25519 /\
                     //x.algID_ed25519 == OID_ED25519 )
                     //length_of_asn1_primitive_TLV x.algID_ed25519 == 5)
-  | _ -> True)
-= match alg with
-  | AlgID_ECDSA_P256 -> ( lemma_serialize_algorithmIdentifier_unfold alg x )
-  | AlgID_Ed25519    -> ( lemma_serialize_algorithmIdentifier_unfold alg x;
+)
+=
+  // match alg with
+  // | AlgID_ECDSA_P256 -> ( lemma_serialize_algorithmIdentifier_unfold alg x )
+  // | AlgID_Ed25519    ->
+                        ( lemma_serialize_algorithmIdentifier_unfold x;
                     assert_norm (length_of_asn1_primitive_TLV x.algID_ed25519 == 5 ))
 
 /// inbound record repr
 let algorithmIdentifier_t_inbound
-  (alg: supported_crypto_alg_t)
-= match alg with
-  | AlgID_ECDSA_P256 -> inbound_sequence_value_of (serialize_algorithmIdentifier alg)
-  | AlgID_Ed25519    -> inbound_sequence_value_of (serialize_algorithmIdentifier alg)
+  // (alg: supported_crypto_alg_t)
+=
+  // match alg with
+  // | AlgID_ECDSA_P256 -> inbound_sequence_value_of (serialize_algorithmIdentifier alg)
+  // | AlgID_Ed25519    ->
+  inbound_sequence_value_of (serialize_algorithmIdentifier)
 
 /// TLV
 // unfold
 let parse_algorithmIdentifier_sequence_TLV
-  (alg: supported_crypto_alg_t)
-: parser (parse_asn1_envelop_tag_with_TLV_kind SEQUENCE) (algorithmIdentifier_t_inbound alg)
-= match alg with
-  | AlgID_ECDSA_P256 -> ( //algorithmIdentifier_t_inbound alg
+  // (alg: supported_crypto_alg_t)
+: parser (parse_asn1_envelop_tag_with_TLV_kind SEQUENCE) (algorithmIdentifier_t_inbound)
+=
+  // match alg with
+  // | AlgID_ECDSA_P256 -> ( //algorithmIdentifier_t_inbound alg
+  //                   //`coerce_parser`
+  //                   parse_asn1_sequence_TLV (serialize_algorithmIdentifier alg) )
+  // | AlgID_Ed25519    -> ( //algorithmIdentifier_t_inbound alg
                     //`coerce_parser`
-                    parse_asn1_sequence_TLV (serialize_algorithmIdentifier alg) )
-  | AlgID_Ed25519    -> ( //algorithmIdentifier_t_inbound alg
-                    //`coerce_parser`
-                    parse_asn1_sequence_TLV (serialize_algorithmIdentifier alg) )
+                    parse_asn1_sequence_TLV (serialize_algorithmIdentifier)
 
 let serialize_algorithmIdentifier_sequence_TLV
-  (alg: supported_crypto_alg_t)
-: serializer (parse_algorithmIdentifier_sequence_TLV alg)
-= match alg with
-  | AlgID_ECDSA_P256 -> ( serialize_asn1_sequence_TLV (serialize_algorithmIdentifier alg) )
-  | AlgID_Ed25519    -> ( serialize_asn1_sequence_TLV (serialize_algorithmIdentifier alg) )
+  // (alg: supported_crypto_alg_t)
+: serializer (parse_algorithmIdentifier_sequence_TLV)
+=
+  // match alg with
+  // | AlgID_ECDSA_P256 -> ( serialize_asn1_sequence_TLV (serialize_algorithmIdentifier alg) )
+  // | AlgID_Ed25519    ->
+  ( serialize_asn1_sequence_TLV (serialize_algorithmIdentifier) )
 
 let lemma_serialize_algorithmIdentifier_sequence_TLV_unfold
-  (alg: supported_crypto_alg_t)
-  (x: algorithmIdentifier_t_inbound alg)
-: Lemma ( predicate_serialize_asn1_sequence_TLV_unfold (serialize_algorithmIdentifier alg) x )
-= lemma_serialize_asn1_sequence_TLV_unfold (serialize_algorithmIdentifier alg) x
+  // (alg: supported_crypto_alg_t)
+  (x: algorithmIdentifier_t_inbound)
+: Lemma ( predicate_serialize_asn1_sequence_TLV_unfold (serialize_algorithmIdentifier) x )
+= lemma_serialize_asn1_sequence_TLV_unfold (serialize_algorithmIdentifier) x
 
 let lemma_serialize_algorithmIdentifier_sequence_TLV_size
-  (alg: supported_crypto_alg_t)
-  (x: algorithmIdentifier_t_inbound alg)
-: Lemma ( predicate_serialize_asn1_sequence_TLV_size (serialize_algorithmIdentifier alg) x )
-= match alg with
-  | AlgID_ECDSA_P256 -> ( lemma_serialize_asn1_sequence_TLV_size (serialize_algorithmIdentifier alg) x )
-  | AlgID_Ed25519    -> ( lemma_serialize_asn1_sequence_TLV_size (serialize_algorithmIdentifier alg) x )
+  // (alg: supported_crypto_alg_t)
+  (x: algorithmIdentifier_t_inbound)
+: Lemma ( predicate_serialize_asn1_sequence_TLV_size (serialize_algorithmIdentifier) x )
+=
+  // match alg with
+  // | AlgID_ECDSA_P256 -> ( lemma_serialize_asn1_sequence_TLV_size (serialize_algorithmIdentifier alg) x )
+  // | AlgID_Ed25519    ->
+  ( lemma_serialize_asn1_sequence_TLV_size (serialize_algorithmIdentifier) x )
 
-#push-options "--z3rlimit 32 --fuel 4 --ifuel 4"
+#push-options "--z3rlimit 32 --fuel 0 --ifuel 0"
 let lemma_serialize_algorithmIdentifier_sequence_TLV_size_exact
-  (alg: supported_crypto_alg_t {alg == AlgID_Ed25519})
-  (x: algorithmIdentifier_t alg)
+  // (alg: supported_crypto_alg_t {alg == AlgID_Ed25519})
+  (x: algorithmIdentifier_t)
 : Lemma (
-  match alg with
+  // match alg with
   // | AlgID_ECDSA_P256 -> ( length_of_opaque_serialization (serialize_algorithmIdentifier_sequence_TLV alg) x == 17 )
-  | AlgID_Ed25519    -> ( lemma_serialize_algorithmIdentifier_size alg x;
-                    length_of_opaque_serialization (serialize_algorithmIdentifier_sequence_TLV alg) x == 7 )
+  // | AlgID_Ed25519    ->
+                   ( lemma_serialize_algorithmIdentifier_size x;
+                    length_of_opaque_serialization (serialize_algorithmIdentifier_sequence_TLV) x == 7 )
 )
-= match alg with
-  | AlgID_Ed25519    -> ( lemma_serialize_algorithmIdentifier_size alg x;
-                    lemma_serialize_asn1_sequence_TLV_unfold (serialize_algorithmIdentifier alg) x;
-                    lemma_serialize_asn1_sequence_TLV_size   (serialize_algorithmIdentifier alg) x;
+=
+  // match alg with
+  // | AlgID_Ed25519    ->
+                  ( lemma_serialize_algorithmIdentifier_size x;
+                    lemma_serialize_asn1_sequence_TLV_unfold (serialize_algorithmIdentifier) x;
+                    lemma_serialize_asn1_sequence_TLV_size   (serialize_algorithmIdentifier) x;
                     // lemma_serialize_algorithmIdentifier_size alg x;
-                    assert_norm (length_of_TLV OID (length_of_opaque_serialization (serialize_algorithmIdentifier alg) x) == 7) )
+                    assert (length_of_TLV OID (length_of_opaque_serialization (serialize_algorithmIdentifier) x) == 7) )
 #pop-options
 
 /// Low
@@ -276,50 +307,54 @@ let lemma_serialize_algorithmIdentifier_sequence_TLV_size_exact
 
 inline_for_extraction
 let serialize32_algorithmIdentifier_backwards
-  (alg: supported_crypto_alg_t)
-: serializer32_backwards (serialize_algorithmIdentifier alg)
-= match alg with
-  | AlgID_ECDSA_P256 -> ( serialize32_synth_backwards
+  // (alg: supported_crypto_alg_t)
+: serializer32_backwards (serialize_algorithmIdentifier)
+=
+  // match alg with
+  // | AlgID_ECDSA_P256 -> ( serialize32_synth_backwards
+  //                   (* ls *) (serialize32_asn1_TLV_backwards_of_type OID
+  //                             `serialize32_nondep_then_backwards`
+  //                             serialize32_asn1_TLV_backwards_of_type OID
+  //                             `serialize32_filter_backwards`
+  //                             filter_algorithmIdentifier_t' alg)
+  //                   (* f2 *) (synth_algorithmIdentifier_t alg)
+  //                   (* g1 *) (synth_algorithmIdentifier_t' alg)
+  //                   (* g1'*) (synth_algorithmIdentifier_t' alg)
+  //                   (* prf*) () )
+  // | AlgID_Ed25519    ->
+                       ( serialize32_synth_backwards
                     (* ls *) (serialize32_asn1_TLV_backwards_of_type OID
-                              `serialize32_nondep_then_backwards`
-                              serialize32_asn1_TLV_backwards_of_type OID
                               `serialize32_filter_backwards`
-                              filter_algorithmIdentifier_t' alg)
-                    (* f2 *) (synth_algorithmIdentifier_t alg)
-                    (* g1 *) (synth_algorithmIdentifier_t' alg)
-                    (* g1'*) (synth_algorithmIdentifier_t' alg)
-                    (* prf*) () )
-  | AlgID_Ed25519    -> ( serialize32_synth_backwards
-                    (* ls *) (serialize32_asn1_TLV_backwards_of_type OID
-                              `serialize32_filter_backwards`
-                              filter_algorithmIdentifier_t' alg)
-                    (* f2 *) (synth_algorithmIdentifier_t alg)
-                    (* g1 *) (synth_algorithmIdentifier_t' alg)
-                    (* g1'*) (synth_algorithmIdentifier_t' alg)
+                              filter_algorithmIdentifier_t')
+                    (* f2 *) (synth_algorithmIdentifier_t)
+                    (* g1 *) (synth_algorithmIdentifier_t')
+                    (* g1'*) (synth_algorithmIdentifier_t')
                     (* prf*) () )
 
 inline_for_extraction
 let serialize32_algorithmIdentifier_sequence_TLV_backwards
-  (alg: supported_crypto_alg_t)
-: serializer32_backwards (serialize_algorithmIdentifier_sequence_TLV alg)
-= match alg with
-  | AlgID_ECDSA_P256 -> ( serialize32_asn1_sequence_TLV_backwards
-                    (* s32 *) (serialize32_algorithmIdentifier_backwards alg) )
-  | AlgID_Ed25519    -> ( serialize32_asn1_sequence_TLV_backwards
-                    (* s32 *) (serialize32_algorithmIdentifier_backwards alg) )
+  // (alg: supported_crypto_alg_t)
+: serializer32_backwards (serialize_algorithmIdentifier_sequence_TLV)
+=
+  // match alg with
+  // | AlgID_ECDSA_P256 -> ( serialize32_asn1_sequence_TLV_backwards
+  //                   (* s32 *) (serialize32_algorithmIdentifier_backwards alg) )
+  // | AlgID_Ed25519    ->
+                        ( serialize32_asn1_sequence_TLV_backwards
+                    (* s32 *) (serialize32_algorithmIdentifier_backwards) )
 
 (* helpers *)
-let _ = assert (length_of_oid OID_EC_GRP_SECP256R1 == 6)
 
 #push-options "--z3rlimit 4 --fuel 0 --ifuel 0"
 noextract inline_for_extraction
-let x509_get_algorithmIdentifier
-  (alg: supported_crypto_alg_t {alg == AlgID_Ed25519})
-: Tot (algorithmIdentifier_t_inbound alg)
+let x509_get_algorithmIdentifier ()
+  // (alg: supported_crypto_alg_t {alg == AlgID_Ed25519})
+: Tot (algorithmIdentifier_t_inbound)
 =
-  match alg with
-  | AlgID_Ed25519 -> ( let algID: algorithmIdentifier_t alg = { algID_ed25519 = OID_ED25519 } in
-                 (* Prf *) lemma_serialize_algorithmIdentifier_size alg algID;
+  // match alg with
+  // | AlgID_Ed25519 ->
+                   ( let algID: algorithmIdentifier_t = { algID_ed25519 = OID_ED25519 } in
+                 (* Prf *) lemma_serialize_algorithmIdentifier_size algID;
                  (* Prf *) (**) lemma_serialize_asn1_oid_TLV_size algID.algID_ed25519;
                  (* return *) algID )
 #pop-options
