src/X509.Crypto.Signature.fst
@@ -14,172 +14,207 @@ module B32 = FStar.Bytes
 open ASN1.Base
 
 let x509_signature_t_aux
-  (alg: supported_crypto_alg_t {alg == AlgID_Ed25519})
-= match alg with
-  | AlgID_Ed25519   -> datatype_of_asn1_type BIT_STRING
+  // (alg: supported_crypto_alg_t {alg == AlgID_Ed25519})
+=
+  // match alg with
+  // | AlgID_Ed25519   ->
+  datatype_of_asn1_type BIT_STRING
 
 let filter_x509_signature
-  (alg: supported_crypto_alg_t {alg == AlgID_Ed25519})
-  (x: x509_signature_t_aux alg)
+  // (alg: supported_crypto_alg_t {alg == AlgID_Ed25519})
+  (x: x509_signature_t_aux)
 : GTot (bool)
-= match alg with
-  | AlgID_Ed25519   -> ( let x = x <: datatype_of_asn1_type BIT_STRING in
+=
+  // match alg with
+  // | AlgID_Ed25519   ->
+  ( let x = x <: datatype_of_asn1_type BIT_STRING in
                    x.bs_len = 65ul &&
                    x.bs_unused_bits = 0ul )
 
 let x509_signature_t
-  (alg: supported_crypto_alg_t {alg == AlgID_Ed25519})
-= match alg with
-  | AlgID_Ed25519   -> ( bs: datatype_of_asn1_type BIT_STRING
+  // (alg: supported_crypto_alg_t {alg == AlgID_Ed25519})
+=
+  // match alg with
+  // | AlgID_Ed25519   ->
+  ( bs: datatype_of_asn1_type BIT_STRING
                        { v bs.bs_len == 65 /\
                          v bs.bs_unused_bits == 0 })
 
 let parse_x509_signature_kind
-  (alg: supported_crypto_alg_t {alg == AlgID_Ed25519})
-= match alg with
-  | AlgID_Ed25519   -> parse_asn1_TLV_kind_of_type BIT_STRING
+  // (alg: supported_crypto_alg_t {alg == AlgID_Ed25519})
+=
+  // match alg with
+  // | AlgID_Ed25519   ->
+  parse_asn1_TLV_kind_of_type BIT_STRING
 
 let parse_x509_signature
-  (alg: supported_crypto_alg_t {alg == AlgID_Ed25519})
-: parser (parse_x509_signature_kind alg) (x509_signature_t alg)
-= match alg with
-  | AlgID_Ed25519   -> ( parse_asn1_TLV_of_type BIT_STRING
+  // (alg: supported_crypto_alg_t {alg == AlgID_Ed25519})
+: parser (parse_x509_signature_kind) (x509_signature_t)
+=
+  // match alg with
+  // | AlgID_Ed25519   ->
+                  ( parse_asn1_TLV_of_type BIT_STRING
                    `parse_filter`
-                   filter_x509_signature alg
+                   filter_x509_signature
                    `parse_synth`
-                   (fun x -> x <: x509_signature_t alg))
+                   (fun x -> x <: x509_signature_t))
 
 let serialize_x509_signature
-  (alg: supported_crypto_alg_t {alg == AlgID_Ed25519})
-: serializer (parse_x509_signature alg)
-= match alg with
-  | AlgID_Ed25519   -> ( serialize_synth
+  // (alg: supported_crypto_alg_t {alg == AlgID_Ed25519})
+: serializer (parse_x509_signature)
+=
+  // match alg with
+  // | AlgID_Ed25519   ->
+                      ( serialize_synth
                    (* p1 *) (parse_asn1_TLV_of_type BIT_STRING
                              `parse_filter`
-                             filter_x509_signature alg)
-                   (* f2 *) (fun x -> x <: x509_signature_t alg)
+                             filter_x509_signature)
+                   (* f2 *) (fun x -> x <: x509_signature_t)
                    (* s1 *) (serialize_asn1_TLV_of_type BIT_STRING
                              `serialize_filter`
-                             filter_x509_signature alg)
-                   (* g1 *) (fun x -> x <: parse_filter_refine (filter_x509_signature alg))
+                             filter_x509_signature)
+                   (* g1 *) (fun x -> x <: parse_filter_refine (filter_x509_signature))
                    (* prf*) () )
 
 let lemma_serialize_x509_signature_unfold
-  (alg: supported_crypto_alg_t {alg == AlgID_Ed25519})
-  (x: x509_signature_t alg)
+  // (alg: supported_crypto_alg_t {alg == AlgID_Ed25519})
+  (x: x509_signature_t)
 : Lemma (
-  match alg with
-  | AlgID_Ed25519   -> ( serialize_x509_signature alg `serialize` x ==
+  // match alg with
+  // | AlgID_Ed25519   ->
+                 ( serialize_x509_signature `serialize` x ==
                    serialize_asn1_TLV_of_type BIT_STRING x )
 )
 = serialize_synth_eq
   (* p1 *) (parse_asn1_TLV_of_type BIT_STRING
             `parse_filter`
-            filter_x509_signature alg)
-  (* f2 *) (fun x -> x <: x509_signature_t alg)
+            filter_x509_signature)
+  (* f2 *) (fun x -> x <: x509_signature_t)
   (* s1 *) (serialize_asn1_TLV_of_type BIT_STRING
             `serialize_filter`
-            filter_x509_signature alg)
-  (* g1 *) (fun x -> x <: parse_filter_refine (filter_x509_signature alg))
+            filter_x509_signature)
+  (* g1 *) (fun x -> x <: parse_filter_refine (filter_x509_signature))
   (* prf*) ()
   (* in *) x
 
 let lemma_serialize_x509_signature_size
-  (alg: supported_crypto_alg_t {alg == AlgID_Ed25519})
-  (x: x509_signature_t alg)
+  // (alg: supported_crypto_alg_t {alg == AlgID_Ed25519})
+  (x: x509_signature_t)
 : Lemma (
-  match alg with
-  | AlgID_Ed25519   -> ( length_of_opaque_serialization (serialize_x509_signature alg) x ==
+  // match alg with
+  // | AlgID_Ed25519   ->
+  ( length_of_opaque_serialization (serialize_x509_signature) x ==
                    length_of_asn1_primitive_TLV #BIT_STRING x /\
-                   length_of_opaque_serialization (serialize_x509_signature alg) x == 67 )
+                   length_of_opaque_serialization (serialize_x509_signature) x == 67 )
 )
-= match alg with
-  | AlgID_Ed25519   -> ( lemma_serialize_x509_signature_unfold alg x;
+=
+  // match alg with
+  // | AlgID_Ed25519   ->
+  ( lemma_serialize_x509_signature_unfold x;
                    lemma_serialize_asn1_bit_string_TLV_size x )
 
 let x509_signature_t_inbound
-  (alg: supported_crypto_alg_t {alg == AlgID_Ed25519})
-= match alg with
-  | AlgID_Ed25519   -> ( inbound_sequence_value_of (serialize_x509_signature alg) )
+  // (alg: supported_crypto_alg_t {alg == AlgID_Ed25519})
+=
+  // match alg with
+  // | AlgID_Ed25519   ->
+  ( inbound_sequence_value_of (serialize_x509_signature) )
 
 let parse_x509_signature_sequence_TLV
-  (alg: supported_crypto_alg_t {alg == AlgID_Ed25519})
-: parser _ (x509_signature_t_inbound alg)
-= match alg with
-  | AlgID_Ed25519   -> ( parse_asn1_sequence_TLV (serialize_x509_signature alg) )
+  // (alg: supported_crypto_alg_t {alg == AlgID_Ed25519})
+: parser _ (x509_signature_t_inbound)
+=
+  // match alg with
+  // | AlgID_Ed25519   ->
+  ( parse_asn1_sequence_TLV (serialize_x509_signature) )
 
 let serialize_x509_signature_sequence_TLV
-  (alg: supported_crypto_alg_t {alg == AlgID_Ed25519})
-: serializer (parse_x509_signature_sequence_TLV alg)
-= match alg with
-  | AlgID_Ed25519   -> ( serialize_asn1_sequence_TLV (serialize_x509_signature alg) )
+  // (alg: supported_crypto_alg_t {alg == AlgID_Ed25519})
+: serializer (parse_x509_signature_sequence_TLV)
+=
+  // match alg with
+  // | AlgID_Ed25519   ->
+  ( serialize_asn1_sequence_TLV (serialize_x509_signature) )
 
 let lemma_serialize_x509_signature_sequence_TLV_unfold
-  (alg: supported_crypto_alg_t {alg == AlgID_Ed25519})
-  (x: x509_signature_t_inbound alg)
-: Lemma ( predicate_serialize_asn1_sequence_TLV_unfold (serialize_x509_signature alg) x )
-= match alg with
-  | AlgID_Ed25519   -> ( lemma_serialize_asn1_sequence_TLV_unfold (serialize_x509_signature alg) x )
+  // (alg: supported_crypto_alg_t {alg == AlgID_Ed25519})
+  (x: x509_signature_t_inbound)
+: Lemma ( predicate_serialize_asn1_sequence_TLV_unfold (serialize_x509_signature) x )
+=
+  // match alg with
+  // | AlgID_Ed25519   ->
+  ( lemma_serialize_asn1_sequence_TLV_unfold (serialize_x509_signature) x )
 
 let lemma_serialize_x509_signature_sequence_TLV_size
-  (alg: supported_crypto_alg_t {alg == AlgID_Ed25519})
-  (x: x509_signature_t_inbound alg)
-: Lemma ( predicate_serialize_asn1_sequence_TLV_size (serialize_x509_signature alg) x )
-= match alg with
-  | AlgID_Ed25519   -> ( lemma_serialize_asn1_sequence_TLV_size (serialize_x509_signature alg) x )
+  // (alg: supported_crypto_alg_t {alg == AlgID_Ed25519})
+  (x: x509_signature_t_inbound)
+: Lemma ( predicate_serialize_asn1_sequence_TLV_size (serialize_x509_signature) x )
+=
+  // match alg with
+  // | AlgID_Ed25519   ->
+  ( lemma_serialize_asn1_sequence_TLV_size (serialize_x509_signature) x )
 
-#push-options "--z3rlimit 32 --fuel 4 --ifuel 4"
+#push-options "--z3rlimit 32 --fuel 0 --ifuel 0"
 let lemma_serialize_x509_signature_sequence_TLV_size_exact
-  (alg: supported_crypto_alg_t {alg == AlgID_Ed25519})
-  (x: x509_signature_t_inbound alg)
+  // (alg: supported_crypto_alg_t {alg == AlgID_Ed25519})
+  (x: x509_signature_t_inbound)
 : Lemma (
-  match alg with
-  | AlgID_Ed25519    -> ( length_of_opaque_serialization (serialize_x509_signature_sequence_TLV alg) x == 69 )
+  // match alg with
+  // | AlgID_Ed25519    ->
+  ( length_of_opaque_serialization (serialize_x509_signature_sequence_TLV) x == 69 )
 )
-= match alg with
-  | AlgID_Ed25519    -> ( lemma_serialize_x509_signature_sequence_TLV_size alg x;
-                    lemma_serialize_x509_signature_size alg x )
+=
+  // match alg with
+  // | AlgID_Ed25519    ->
+  ( lemma_serialize_x509_signature_sequence_TLV_size x;
+                    lemma_serialize_x509_signature_size x )
 #pop-options
 
 (* Low *)
 inline_for_extraction
 let serialize32_x509_signature_backwards
-  (alg: supported_crypto_alg_t {alg == AlgID_Ed25519})
-: serializer32_backwards (serialize_x509_signature alg)
-= match alg with
-  | AlgID_Ed25519   -> ( serialize32_synth_backwards
+  // (alg: supported_crypto_alg_t {alg == AlgID_Ed25519})
+: serializer32_backwards (serialize_x509_signature)
+=
+  // match alg with
+  // | AlgID_Ed25519   ->
+                       ( serialize32_synth_backwards
                    (* s32 *) (serialize32_asn1_bit_string_TLV_backwards ()
                               `serialize32_filter_backwards`
-                              filter_x509_signature alg)
-                   (* f2  *) (fun x -> x <: x509_signature_t alg)
-                   (* g1  *) (fun x -> x <: parse_filter_refine (filter_x509_signature alg))
-                   (* g1' *) (fun x -> x <: parse_filter_refine (filter_x509_signature alg))
+                              filter_x509_signature)
+                   (* f2  *) (fun x -> x <: x509_signature_t)
+                   (* g1  *) (fun x -> x <: parse_filter_refine (filter_x509_signature))
+                   (* g1' *) (fun x -> x <: parse_filter_refine (filter_x509_signature))
                    (* prf *) () )
 
 inline_for_extraction
 let serialize32_x509_signature_sequence_TLV_backwards
-  (alg: supported_crypto_alg_t {alg == AlgID_Ed25519})
-: serializer32_backwards (serialize_x509_signature_sequence_TLV alg)
-= match alg with
-  | AlgID_Ed25519   -> ( serialize32_asn1_sequence_TLV_backwards (serialize32_x509_signature_backwards alg) )
+  // (alg: supported_crypto_alg_t {alg == AlgID_Ed25519})
+: serializer32_backwards (serialize_x509_signature_sequence_TLV)
+=
+  // match alg with
+  // | AlgID_Ed25519   ->
+  ( serialize32_asn1_sequence_TLV_backwards (serialize32_x509_signature_backwards) )
 
 
 (* Helpers *)
-let _ = assert (length_of_oid OID_EC_GRP_SECP256R1 == 6)
 
 module B32 = FStar.Bytes
 let x509_signature_raw_t
-  (alg: supported_crypto_alg_t {alg == AlgID_Ed25519})
-= match alg with
-  | AlgID_Ed25519   -> ( B32.lbytes32 64ul )
+  // (alg: supported_crypto_alg_t {alg == AlgID_Ed25519})
+=
+  // match alg with
+  // | AlgID_Ed25519   ->
+  ( B32.lbytes32 64ul )
 
 inline_for_extraction noextract
 let x509_get_signature
-  (alg: supported_crypto_alg_t {alg == AlgID_Ed25519})
-  (sig32: x509_signature_raw_t alg)
-: Tot (x509_signature_t_inbound alg)
+  // (alg: supported_crypto_alg_t {alg == AlgID_Ed25519})
+  (sig32: x509_signature_raw_t)
+: Tot (x509_signature_t_inbound)
 =
-  match alg with
-  | AlgID_Ed25519   -> ( let sig_bs: x509_signature_t alg = Mkbit_string_t 65ul 0ul sig32 in
-                   (* Prf *) lemma_serialize_x509_signature_size alg sig_bs;
+  // match alg with
+  // | AlgID_Ed25519   ->
+  ( let sig_bs: x509_signature_t = Mkbit_string_t 65ul 0ul sig32 in
+                   (* Prf *) lemma_serialize_x509_signature_size sig_bs;
                    (* return *) sig_bs )
