src/RIoT.X509.Base.fst
@@ -1,8 +1,8 @@
 module RIoT.X509.Base
 open X509.Base
 
-inline_for_extraction
-let alg_DeviceID = AlgID_Ed25519
+// inline_for_extraction
+// let alg_DeviceID = AlgID_Ed25519
 
-inline_for_extraction
-let alg_AliasKey = AlgID_Ed25519
+// inline_for_extraction
+// let alg_AliasKey = AlgID_Ed25519
